To prove an implication <span class="ntb">P ⇒ Q</span>, it is enough to assume <span class="ntb">P</span>, and from it, deduce <span class="ntb">Q</span>.

Perhaps a better way to say this is that to prove a statement of the form <span class="ntb">P ⇒ Q</span> directly, you must explain why <span class="ntb">Q</span> is <span class="gtb">true</span>, but you get to assume <span class="ntb">P</span> is <span class="gtb">true</span> first. After all, you only care about whether <span class="ntb">Q</span> is <span class="gtb">true</span> in the case that <span class="ntb">P</span> is as well.

Suppose the numbers <span class="ntb">a</span> and <span class="ntb">b</span> are even. This means that <span class="ntb">a = 2k</span> and <span class="ntb">b = 2j</span> for some integers <span class="ntb">k</span> and <span class="ntb">j</span>. The sum is then <span class="ntb">a + b = 2k + 2j = 2(k + j)</span>.

Since <span class="ntb">k + j</span> is an integer, this means that <span class="ntb">a + b</span> is even.