

<span class="btb">Two statements x and y</span> are called <span class="gtb">equivalent</span> if and only if their truth values for all possible truth value assignments of the atomic statements in x and y are the same. In this case, we write <span class="btb">x ≡ y</span> and also say that x and y are <span class="gtb">equivalent</span>.

**Example: Assertion:** <span class="btb">(x ⇔ y) ≡ (¬x ∨ y)</span>

| <span class="btb">x</span> | <span class="btb">y</span> | <span class="btb">¬x</span> | <span class="btb">x ⇒ y</span> | <span class="btb">¬x ∨ y</span> |
|---|---|---|---|---|
| <span class="rtb">F</span> | <span class="rtb">F</span> | <span class="gtb">T</span> | <span class="gtb">T</span> | <span class="gtb">T</span> |
| <span class="rtb">F</span> | <span class="gtb">T</span> | <span class="gtb">T</span> | <span class="gtb">T</span> | <span class="gtb">T</span> |
| <span class="gtb">T</span> | <span class="rtb">F</span> | <span class="rtb">F</span> | <span class="rtb">F</span> | <span class="rtb">F</span> |
| <span class="gtb">T</span> | <span class="gtb">T</span> | <span class="rtb">F</span> | <span class="gtb">T</span> | <span class="gtb">T</span> |